heap_lang/lib/counter.v
@@ -1,7 +1,7 @@
 From iris.program_logic Require Export weakestpre.
 From iris.heap_lang Require Export lang.
 From iris.proofmode Require Import tactics.
-From iris.program_logic Require Import auth.
+From iris.algebra Require Import auth.
 From iris.heap_lang Require Import proofmode notation.
 
 Definition newcounter : val := λ: <>, ref #0.
@@ -13,20 +13,21 @@ Definition read : val := λ: "l", !"l".
 Global Opaque newcounter inc get.
 
 (** The CMRA we need. *)
-Class counterG Σ := CounterG { counter_tokG :> authG Σ mnatUR }.
-Definition counterΣ : gFunctors := #[authΣ mnatUR].
+Class counterG Σ := CounterG { counter_tokG :> inG Σ (authR mnatUR) }.
+Definition counterΣ : gFunctors := #[GFunctor (constRF (authR mnatUR))].
 
 Instance subG_counterΣ {Σ} : subG counterΣ Σ → counterG Σ.
-Proof. intros [? _]%subG_inv. split; apply _. Qed.
+Proof. intros [?%subG_inG _]%subG_inv. split; apply _. Qed.
 
 Section proof.
 Context `{!heapG Σ, !counterG Σ} (N : namespace).
 
-Definition counter_inv (l : loc) (n : mnat) : iProp Σ := (l ↦ #n)%I.
+Definition counter_inv (γ : gname) (l : loc) : iProp Σ :=
+  (∃ n, own γ (● (n : mnat)) ★ l ↦ #n)%I.
 
 Definition counter (l : loc) (n : nat) : iProp Σ :=
   (∃ γ, heapN ⊥ N ∧ heap_ctx ∧
-        auth_ctx γ N (counter_inv l) ∧ auth_own γ (n:mnat))%I.
+        inv N (counter_inv γ l) ∧ own γ (◯ (n : mnat)))%I.
 
 (** The main proofs. *)
 Global Instance counter_persistent l n : PersistentP (counter l n).
@@ -37,35 +38,33 @@ Lemma newcounter_spec (R : iProp Σ) Φ :
   heap_ctx ★ (∀ l, counter l 0 -★ Φ #l) ⊢ WP newcounter #() {{ Φ }}.
 Proof.
   iIntros (?) "[#Hh HΦ]". rewrite /newcounter /=. wp_seq. wp_alloc l as "Hl".
-  iVs (auth_alloc (counter_inv l) N _ (O:mnat) with "[Hl]")
-    as (γ) "[#? Hγ]"; try by auto.
+  iVs (own_alloc (● (O:mnat) ⋅ ◯ (O:mnat))) as (γ) "[Hγ Hγ']"; first done.
+  iVs (inv_alloc N _ (counter_inv γ l) with "[Hl Hγ]").
+  { iNext. iExists 0%nat. by iFrame. }
   iVsIntro. iApply "HΦ". rewrite /counter; eauto 10.
 Qed.
 
-Lemma inc_spec l j (Φ : val → iProp Σ) :
-  counter l j ★ (counter l (S j) -★ Φ #()) ⊢ WP inc #l {{ Φ }}.
+Lemma inc_spec l n (Φ : val → iProp Σ) :
+  counter l n ★ (counter l (S n) -★ Φ #()) ⊢ WP inc #l {{ Φ }}.
 Proof.
   iIntros "[Hl HΦ]". iLöb as "IH". wp_rec.
-  iDestruct "Hl" as (γ) "(% & #? & #Hγ & Hγf)".
-  wp_bind (! _)%E.
-  iVs (auth_open (counter_inv l) with "[Hγf]") as (j') "(% & Hl & Hclose)"; auto.
-  rewrite {2}/counter_inv.
-  wp_load. iVs ("Hclose" $! j with "[Hl]") as "Hγf"; eauto.
-  iVsIntro. wp_let; wp_op. wp_bind (CAS _ _ _).
-  iVs (auth_open (counter_inv l) with "[Hγf]") as (j'') "(% & Hl & Hclose)"; auto.
-  rewrite {2}/counter_inv.
-  destruct (decide (j `max` j'' = j `max` j')) as [Hj|Hj].
-  - wp_cas_suc; first (by do 3 f_equal).
-    iVs ("Hclose" $! (1 + j `max` j')%nat with "[Hl]") as "Hγf".
-    { iSplit; [iPureIntro|iNext].
-      { apply mnat_local_update. abstract lia. }
-      rewrite {2}/counter_inv !mnat_op_max (Nat.max_l (S _)); last abstract lia.
-      by rewrite Nat2Z.inj_succ -Z.add_1_l. }
-    iVsIntro. wp_if.
-    iVsIntro; iApply "HΦ"; iExists γ; repeat iSplit; eauto.
-    iApply (auth_own_mono with "Hγf"). apply mnat_included. abstract lia.
-  - wp_cas_fail; first (rewrite !mnat_op_max; by intros [= ?%Nat2Z.inj]).
-    iVs ("Hclose" $! j with "[Hl]") as "Hγf"; eauto.
+  iDestruct "Hl" as (γ) "(% & #? & #Hinv & Hγf)".
+  wp_bind (! _)%E. iInv N as (c) ">[Hγ Hl]" "Hclose".
+  wp_load. iVs ("Hclose" with "[Hl Hγ]") as "_"; [iNext; iExists c; by iFrame|].
+  iVsIntro. wp_let. wp_op.
+  wp_bind (CAS _ _ _). iInv N as (c') ">[Hγ Hl]" "Hclose".
+  destruct (decide (c' = c)) as [->|].
+  - iDestruct (own_valid_2 with "[$Hγ $Hγf]")
+      as %[?%mnat_included _]%auth_valid_discrete_2.
+    iVs (own_update_2 with "[$Hγ $Hγf]") as "[Hγ Hγf]".
+    { apply auth_update, (mnat_local_update _ _ (S c)); auto. } 
+    wp_cas_suc. iVs ("Hclose" with "[Hl Hγ]") as "_".
+    { iNext. iExists (S c). rewrite Nat2Z.inj_succ Z.add_1_l. by iFrame. }
+    iVsIntro. wp_if. iApply "HΦ"; iExists γ; repeat iSplit; eauto.
+    iApply (own_mono with "Hγf"). apply: auth_frag_mono.
+    by apply mnat_included, le_n_S.
+  - wp_cas_fail; first (by intros [= ?%Nat2Z.inj]).
+    iVs ("Hclose" with "[Hl Hγ]") as "_"; [iNext; iExists c'; by iFrame|].
     iVsIntro. wp_if. iApply ("IH" with "[Hγf] HΦ"). rewrite {3}/counter; eauto 10.
 Qed.
 
@@ -73,15 +72,13 @@ Lemma read_spec l j (Φ : val → iProp Σ) :
   counter l j ★ (∀ i, ■ (j ≤ i)%nat → counter l i -★ Φ #i)
   ⊢ WP read #l {{ Φ }}.
 Proof.
-  iIntros "[Hc HΦ]". iDestruct "Hc" as (γ) "(% & #? & #Hγ & Hγf)".
-  rewrite /read /=. wp_let.
-  iVs (auth_open (counter_inv l) with "[Hγf]") as (j') "(% & Hl & Hclose)"; auto.
-  wp_load.
-  iVs ("Hclose" $! (j `max` j') with "[Hl]") as "Hγf".
-  { iSplit; [iPureIntro|iNext].
-    { apply mnat_local_update; abstract lia. }
-    by rewrite !mnat_op_max -Nat.max_assoc Nat.max_idempotent. }
-  iVsIntro. rewrite !mnat_op_max.
-  iApply ("HΦ" with "[%]"); first abstract lia. rewrite /counter; eauto 10.
+  iIntros "[Hc HΦ]". iDestruct "Hc" as (γ) "(% & #? & #Hinv & Hγf)".
+  rewrite /read /=. wp_let. iInv N as (c) ">[Hγ Hl]" "Hclose". wp_load.
+  iDestruct (own_valid_2 with "[$Hγ $Hγf]")
+    as %[?%mnat_included _]%auth_valid_discrete_2.
+  iVs (own_update_2 with "[$Hγ $Hγf]") as "[Hγ Hγf]".
+  { apply auth_update, (mnat_local_update _ _ c); auto. }
+  iVs ("Hclose" with "[Hl Hγ]") as "_"; [iNext; iExists c; by iFrame|].
+  iApply ("HΦ" with "[%]"); rewrite /counter; eauto 10.
 Qed.
 End proof.
